Add notations for commands and types. Also create sample programs

PyLevelLang/src/PyLevelLang/Notations.v
@@ -7,10 +7,10 @@ Require Import Coq.Lists.List.
 Import ListNotations.
 Import ResultMonadNotations.
 
-(* Set Printing All. *)
-
-Declare Custom Entry pylevel.
 Declare Scope pylevel_scope.
+Declare Custom Entry py_expr.
+Declare Custom Entry py_comm.
+Declare Custom Entry py_type.
 
 Local Open Scope Z_scope.
 Local Open Scope string_scope.
@@ -24,124 +24,209 @@ Coercion PAInt : Z >-> patom.
 Coercion PABool : bool >-> patom.
 Coercion PEAtom : patom >-> pexpr.
 
-Notation "<{ e }>"       := (e : pexpr) (at level 0, e custom pylevel at level 99, only parsing) : pylevel_scope.
-Notation "<{ e }>"       := e (at level 0, e custom pylevel at level 99, only printing) : pylevel_scope.
-Notation "<[ e ]>"       := e (in custom pylevel at level 0, e constr at level 200) : pylevel_scope.
-Notation "( x )"         := x (in custom pylevel at level 0, x custom pylevel at level 99) : pylevel_scope.
-Notation "x"             := x (in custom pylevel at level 0, x constr at level 0) : pylevel_scope.
+Notation "<{ e }>"       := (e : pcommand) (at level 0, e custom py_comm at level 99, only parsing) : pylevel_scope.
+Notation "<{ e }>"       := e (at level 0, e custom py_comm at level 99, only printing) : pylevel_scope.
+(*
+Notation "<{ e }>"       := (e : pexpr) (at level 0, e custom py_expr at level 99, only parsing) : pylevel_scope.
+Notation "<{ e }>"       := e (at level 0, e custom py_expr at level 99, only printing) : pylevel_scope.
+ *)
+
+Notation "<[ e ]>"       := e (in custom py_expr at level 0, e constr at level 200) : pylevel_scope.
+Notation "<[ e ]>"       := e (in custom py_comm at level 0, e constr at level 200) : pylevel_scope.
+Notation "<[ e ]>"       := e (in custom py_type at level 0, e constr at level 200) : pylevel_scope.
+Notation "( x )"         := x (in custom py_expr at level 0, x custom py_expr at level 99) : pylevel_scope.
+Notation "( x )"         := x (in custom py_comm at level 0, x custom py_comm at level 99) : pylevel_scope.
+Notation "( x )"         := x (in custom py_type at level 0, x custom py_type at level 99) : pylevel_scope.
+Notation "x"             := x (in custom py_expr at level 0, x constr at level 0) : pylevel_scope.
+Notation "x"             := x (in custom py_comm at level 0, x constr at level 0) : pylevel_scope.
+Notation "x"             := x (in custom py_type at level 0, x constr at level 0) : pylevel_scope.
 
 (* TODO Allow string constants (which are different from vars) *)
 
+(* Command parsing *)
+Notation "'skip'"                     := (PCSkip)
+   (in custom py_comm at level 0) : pylevel_scope.
+Notation "c ; "                    := c
+   (in custom py_comm at level 90) : pylevel_scope.
+Notation "c1 ; c2"                    := (PCSeq c1 c2)
+   (in custom py_comm at level 90, c1 custom py_comm, c2 custom py_comm) : pylevel_scope.
+Notation "'let' x := p 'in' c"        := (PCLet x p c)
+   (in custom py_comm at level 100, p custom py_expr, c custom py_comm) : pylevel_scope.
+Notation "'let' 'mut' x := p 'in' c"    := (PCLetMut x%string p c)
+   (in custom py_comm at level 100, p custom py_expr, c custom py_comm) : pylevel_scope.
+Notation "x <- p"                     := (PCGets x p)
+   (in custom py_comm at level 50, p custom py_expr) : pylevel_scope.
+Notation "'if' p 'then' c1 'else' c2 'end'" := (PCIf p c1 c2)
+   (in custom py_comm at level 80, p custom py_expr, c1 custom py_comm, c2 custom py_comm) : pylevel_scope.
+Notation "'for' 'each' x 'in' p : c 'end'"  := (PCForeach x p c)
+   (in custom py_comm at level 80, p custom py_expr, c custom py_comm) : pylevel_scope.
+
+(* Type parsing (Types are prefixed with @ so they do not become keywords and pollute the namespace *)
+Notation "@ 'int'"         := TInt (in custom py_type at level 99) : pylevel_scope.
+Notation "@ 'bool'"        := TBool (in custom py_type at level 99) : pylevel_scope.
+Notation "@ 'string'"      := TString (in custom py_type at level 99) : pylevel_scope.
+Notation "@ 'pair' s x y"  := (TPair s%string x y) (in custom py_type at level 99) : pylevel_scope.
+Notation "@ 'empty'"       := TEmpty (in custom py_type at level 99) : pylevel_scope.
+Notation "@ 'list' t"      := (TList t) (in custom py_type at level 99) : pylevel_scope.
+
+
+(* Expression parsing *)
+
 (* Unary operations (PEUnop) *)
 Notation "- x"         := (PEUnop PONeg x)
-   (in custom pylevel at level 10) : pylevel_scope.
+   (in custom py_expr at level 10) : pylevel_scope.
 Notation "! x"         := (PEUnop PONot x)
-   (in custom pylevel at level 10) : pylevel_scope.
+   (in custom py_expr at level 10) : pylevel_scope.
 Notation "'length(' x ')'"   := (PEUnop POLength x)
-   (in custom pylevel at level 10) : pylevel_scope.
+   (in custom py_expr at level 10) : pylevel_scope.
 
 
 (* not a unary operator, move *)
-Notation "x [ field ]"        := (PEProj x field%string) (in custom pylevel at level 10) : pylevel_scope.
+Notation "x [ field ]"        := (PEProj x field%string) (in custom py_expr at level 10) : pylevel_scope.
 (* syntactic sugar *)
-Notation "'fst(' x ')'" := <{ x["0"] }>
-   (in custom pylevel at level 10, format "fst( x )") : pylevel_scope.
-Notation "'snd(' x ')'" := <{ x["1"] }>
-   (in custom pylevel at level 10) : pylevel_scope.
+Notation "'fst(' x ')'" := (PEProj x "0")
+   (in custom py_expr at level 10, format "fst( x )") : pylevel_scope.
+Notation "'snd(' x ')'" := (PEProj x "1")
+   (in custom py_expr at level 10) : pylevel_scope.
 
 
 (* Binary operators (PEBinop) *)
 Notation "x + y"              := (PEBinop POPlus x y)
-   (in custom pylevel at level 50, left associativity) : pylevel_scope.
+   (in custom py_expr at level 50, left associativity) : pylevel_scope.
 Notation "x - y"              := (PEBinop POMinus x y)
-   (in custom pylevel at level 50, left associativity) : pylevel_scope.
+   (in custom py_expr at level 50, left associativity) : pylevel_scope.
 Notation "x * y"              := (PEBinop POTimes x y)
-   (in custom pylevel at level 40, left associativity) : pylevel_scope.
+   (in custom py_expr at level 40, left associativity) : pylevel_scope.
 Notation "x / y"              := (PEBinop PODiv x y)
-   (in custom pylevel at level 40, left associativity) : pylevel_scope.
+   (in custom py_expr at level 40, left associativity) : pylevel_scope.
 Notation "x % y"              := (PEBinop POMod x y)
-   (in custom pylevel at level 40, left associativity) : pylevel_scope.
+   (in custom py_expr at level 40, left associativity) : pylevel_scope.
 Notation "x && y"             := (PEBinop POAnd x y)
-   (in custom pylevel at level 40, left associativity) : pylevel_scope.
+   (in custom py_expr at level 40, left associativity) : pylevel_scope.
 Notation "x || y"             := (PEBinop POOr x y)
-   (in custom pylevel at level 50, left associativity) : pylevel_scope.
+   (in custom py_expr at level 50, left associativity) : pylevel_scope.
 Notation "x ++ y"             := (PEBinop POConcat x y)
-   (in custom pylevel at level 60, left associativity) : pylevel_scope.
+   (in custom py_expr at level 60, left associativity) : pylevel_scope.
 Notation "x < y"              := (PEBinop POLess x y)
-   (in custom pylevel at level 70, left associativity) : pylevel_scope.
+   (in custom py_expr at level 70, left associativity) : pylevel_scope.
 Notation "x == y"             := (PEBinop POEq x y)
-   (in custom pylevel at level 70, left associativity) : pylevel_scope.
+   (in custom py_expr at level 70, left associativity) : pylevel_scope.
 Notation "'repeat(' list ',' cnt ')'"       := (PEBinop PORepeat list cnt)
-   (in custom pylevel at level 10, left associativity) : pylevel_scope.
+   (in custom py_expr at level 10, left associativity) : pylevel_scope.
 Notation "( x , y )"          := (PEBinop POPair x y)
-   (in custom pylevel at level 0, x custom pylevel at level 99,
-    y custom pylevel at level 99, left associativity) : pylevel_scope.
+   (in custom py_expr at level 0, x custom py_expr at level 99,
+    y custom py_expr at level 99, left associativity) : pylevel_scope.
 Notation "x :: y"             := (PEBinop POCons x y)
-   (in custom pylevel at level 55, right associativity) : pylevel_scope.
+   (in custom py_expr at level 55, right associativity) : pylevel_scope.
 Notation "'range(' x ',' y ')'"  := (PEBinop PORange x y)
-   (in custom pylevel at level 10, left associativity) : pylevel_scope.
+   (in custom py_expr at level 10, left associativity) : pylevel_scope.
 
 Notation "[ x , .. , y , z ]"   := (PEBinop POCons x .. (PEBinop POCons y (PESingleton z)) ..)
-   (in custom pylevel at level 0, left associativity) : pylevel_scope.
+   (in custom py_expr at level 0, left associativity) : pylevel_scope.
 Notation "[ x ]"                := (PESingleton x)
-   (in custom pylevel at level 0) : pylevel_scope.
+   (in custom py_expr at level 0) : pylevel_scope.
 Notation "'nil(' t ')'"        := (PANil t)
-   (in custom pylevel at level 10) : pylevel_scope.
+   (in custom py_expr at level 10, t custom py_type) : pylevel_scope.
 
 
 (* Other pexpr *)
 Notation "'flatmap' e1 x e2"           := (PEFlatmap e1 x%string e2)
-   (in custom pylevel at level 99, x constr at level 0) : pylevel_scope.
+   (in custom py_expr at level 99, x constr at level 0) : pylevel_scope.
 Notation "'if' p1 'then' p2 'else' p3" := (PEIf p1 p2 p3)
-   (in custom pylevel at level 99) : pylevel_scope.
+   (in custom py_expr at level 99) : pylevel_scope.
 Notation "'let' x := p1 'in' p2"       := (PELet x p1 p2)
-   (in custom pylevel at level 99) : pylevel_scope.
+   (in custom py_expr at level 99) : pylevel_scope.
 (* TODO PERecord *)
 
 Section Tests.
-   Goal <{ -3 }> = PEUnop PONeg 3. reflexivity. Abort.
-   Goal <{ -(3) }> = PEUnop PONeg 3. reflexivity. Abort.
+   Goal <{ skip }> = PCSkip. reflexivity. Abort.
+   Goal <{ skip; }> = PCSkip. reflexivity. Abort.
+   Goal <{ skip; skip }> = PCSeq PCSkip PCSkip. reflexivity. Abort.
 
-   Goal <{ !true }> = PEUnop PONot true. reflexivity. Abort.
-   Goal <{ !(true) }> = PEUnop PONot true. reflexivity. Abort.
+   Goal <{ "x" <- 0 }> = PCGets "x" (PEAtom 0). reflexivity. Abort.
 
-   Goal <{ fst(0) }> = PEProj 0 "0". reflexivity. Abort.
-   Goal forall x, <{ x["0"] }> = PEProj x "0". reflexivity. Abort.
+   Goal <{ "_" <- -3 }> = PCGets "_" (PEUnop PONeg 3). reflexivity. Abort.
+   Goal <{ "_" <- -(3) }> = PCGets "_" (PEUnop PONeg 3). reflexivity. Abort.
 
-   Goal <{ ((1 + 3)*4, 2) }> = (PEBinop POPair (PEBinop POTimes (PEBinop POPlus 1 3) 4) 2).
+   Goal <{ "_" <- !true }> = PCGets "_" (PEUnop PONot true). reflexivity. Abort.
+   Goal <{ "_" <- !(true) }> = PCGets "_" (PEUnop PONot true). reflexivity. Abort.
+
+   Goal <{ "_" <- length([ 1, 2, 3]) }> = PCGets "_"
+     (PEUnop POLength (PEBinop POCons 1 (PEBinop POCons 2 (PESingleton 3)))).
    reflexivity. Abort.
 
-   Goal <{ [1, 2, 3] }> = PEBinop POCons 1 (PEBinop POCons 2 (PESingleton 3)).
+   Goal <{ "_" <- fst(0) }> = PCGets "_" (PEProj 0 "0"). reflexivity. Abort.
+   Goal forall x, <{ "_" <- x["0"] }> = PCGets "_" (PEProj x "0"). reflexivity. Abort.
+
+   Goal <{ "_" <- ((1 + 3)*4, 2) }> = PCGets "_" ((PEBinop POPair (PEBinop POTimes (PEBinop POPlus 1 3) 4) 2)).
    reflexivity. Abort.
 
-   Goal <{ [1, 2] }> = PEBinop POCons 1 (PESingleton 2).
+   Goal <{ "_" <- [1, 2, 3] }> = PCGets "_" (PEBinop POCons 1 (PEBinop POCons 2 (PESingleton 3))).
    reflexivity. Abort.
 
-   Goal <{ [ 1 ] }> = PESingleton 1.
+   Goal <{ "_" <- [1, 2] }> = PCGets "_" (PEBinop POCons 1 (PESingleton 2)).
    reflexivity. Abort.
 
-   Goal <{ true }> = PEAtom (PABool true).
+   Goal <{ "_" <- true }> = PCGets "_" (PEAtom (PABool true)).
    reflexivity. Abort.
 
-   Goal <{ 1 :: 2 :: [3, 4] }> = PEBinop POCons 1 (PEBinop POCons 2 (PEBinop POCons 3 (PESingleton 4))).
+   Goal <{ "_" <- [ 1 ] }> = PCGets "_" (PESingleton 1).
    reflexivity. Abort.
+
+   Goal <{ "_" <- true }> = PCGets "_" (PEAtom (PABool true)).
+   reflexivity. Abort.
+
+   Goal <{ "_" <- 1 :: 2 :: [3, 4] }> = PCGets "_"
+      (PEBinop POCons 1 (PEBinop POCons 2 (PEBinop POCons 3 (PESingleton 4)))).
+   reflexivity. Abort.
+
+   Goal <{ "_" <- 3 :: 4 :: nil(@int) }> = PCGets "_"
+      (PEBinop POCons 3 (PEBinop POCons 4 (PANil TInt))).
+   reflexivity. Abort.
+   Goal <{ "_" <- true :: false :: nil(@bool) }> = PCGets "_"
+      (PEBinop POCons true (PEBinop POCons false (PANil TBool))).
+   reflexivity. Abort.
+   Goal <{ "_" <- [2,4] :: nil(@list @int) }> = PCGets "_"
+      (PEBinop POCons (PEBinop POCons 2 (PESingleton 4)) (PANil (TList TInt))).
+   reflexivity. Abort.
+
+   (* TODO Is this how the precedence should be for let? *)
+   Goal <{ let "x" := 3 + 4 in "y" <- "x"+1; "z" <- 5+"x" }> =
+      (PCLet "x" (PEBinop POPlus 3 4)
+         (PCSeq (PCGets "y" (PEBinop POPlus "x" 1))
+                (PCGets "z" (PEBinop POPlus 5 "x")))).
+   reflexivity. Abort.
+
+   Goal <{ (let mut "x" := 3 in "y" <- "x" + 1);
+           "x" <- "y" * 2;
+           skip }> =
+           PCSeq (
+             PCSeq (PCLetMut "x" 3 (PCGets "y" (PEBinop POPlus "x" 1)))
+                   (PCGets "x" (PEBinop POTimes "y" 2))
+                 )
+             PCSkip.
+   reflexivity. Abort.
+
+
+   Goal <{ if 3 == 3 then "y" <- 0+1 else "y" <- 0+10; "a" <- 0; end }> =
+      PCIf (PEBinop POEq 3 3)
+           (PCGets "y" (PEBinop POPlus 0 1))
+           (PCSeq (PCGets "y" (PEBinop POPlus 0 10))
+                  (PCGets "a" 0)).
+   reflexivity. Abort.
+
+   Goal <{ for each "x" in [1,2]++[3]:
+             "a" <- "x"*2;
+             "b" <- "x"+1
+           end;
+           "z" <- 123 }> =
+         PCSeq (PCForeach "x" (PEBinop POConcat (PEBinop POCons 1 (PESingleton 2)) (PESingleton 3))
+                  (PCSeq (PCGets "a" (PEBinop POTimes "x" 2))
+                         (PCGets "b" (PEBinop POPlus "x" 1))))
+               (PCGets "z" 123).
+   reflexivity. Abort.
+
 End Tests.
-
-
-
-
-(* pcommand *)
-(*
-Notation "'done'"                     := (PCSkip) (in custom pylevel at level 99) : pylevel_scope.
-Notation "c1 ; c2"                    := (PCSeq c1 c2) (in custom pylevel at level 99) : pylevel_scope.
-Notation "'let' x := p 'in' c"        := (PCLet x p c) (in custom pylevel at level 99) : pylevel_scope.
-Notation "'let mut' x := p 'in' c"    := (PCLetMut x p c) (in custom pylevel at level 99) : pylevel_scope.
-Notation "x <- p"          := (PCGets x p) (in custom pylevel at level 99) : pylevel_scope.
-Notation "'if' p 'then' c1 'else' c2" := (PCIf p c1 c2) (in custom pylevel at level 99) : pylevel_scope.
-Notation "'for' 'each' x 'in' p : c"  := (PCForeach x p c) (in custom pylevel at level 99) : pylevel_scope.
-*)
-
-
 
 Unset Printing All.
 
@@ -152,43 +237,129 @@ Section Examples.
   Instance locals : map.map string {t & interp_type t} := SortedListString.map _.
   Instance locals_ok : map.ok locals := SortedListString.ok _.
 
-  Definition elaborate_interpret (l : locals) (p : pexpr) : result {t & interp_type t} :=
-    e <- elaborate (map.map_values (fun x => (projT1 x, true)) l) p;;
-    Success (existT _ _ (interp_expr l (projT2 e))).
+  Definition elaborate_interpret (l : locals) (pc : pcommand) : result locals :=
+    c <- elaborate_command (map.map_values (fun x => (projT1 x, true)) l) pc;;
+    Success (interp_command l c).
 
-  (*
-  Set Printing All.
-  Definition c1 := <{ let "a" := (1) in (if (1 > 1) then 3 else 4) }>.
-  Print c1.
-   *)
+  Definition set_local (l : locals) {t : type} (x : string) (v : interp_type t) :
+    locals := map.put l x (existT _ _ v).
 
-  Goal elaborate_interpret map.empty <{ 1 + 2 }> = Success (existT _ (TInt) (3)).
-  Proof. reflexivity. Abort.
+  Fixpoint init_locals (vars : list string) :=
+     match vars with
+     | [] => map.empty
+     | x :: xs => @set_local (init_locals xs) TInt x(0)
+     end.
 
-  Goal elaborate_interpret map.empty <{ let "x" := 2 in "x" }> = Success (existT _ (TInt) (2)).
-  Proof. reflexivity. Abort.
+  Definition run_program (init : locals) (pc : pcommand) :=
+   match elaborate_interpret init pc with
+       | Success x => Success x.(SortedList.value)
+       | Failure e => Failure e
+       end.
 
-  Goal elaborate_interpret map.empty <{ let "x" := 2 in "x"+3*100 }> = Success (existT _ (TInt) (302)).
-  Proof. reflexivity. Abort.
-
-  Goal elaborate_interpret map.empty <{ ! (1 == 1)  }> = Success (existT _ (TBool) (false)).
-  Proof. reflexivity. Abort.
-
-  Goal elaborate_interpret map.empty <{ if !(1 == 2) then 5 else 98+1 }> = Success (existT _ (TInt) (5)).
-  Proof. reflexivity. Abort.
-
-  Goal elaborate_interpret map.empty <{ range(3, 5) }> = Success (existT _ (TList TInt) (3 :: 4 :: nil)).
-  Proof. reflexivity. Abort.
-
-  Goal elaborate_interpret map.empty <{ flatmap [1, 2] "x" ["x"]}> = Success (existT _ (TList TInt) (1 :: 2 :: nil)).
-  reflexivity. Abort.
-
-  Goal elaborate_interpret map.empty <{ flatmap [1] "x" ["x"] }> = Success (existT _ (TList TInt) (1 :: nil)).
+  Goal run_program (init_locals ["a"]) <{ "a" <- 5; }> = Success [("a", existT interp_type TInt 5)].
   reflexivity.  Abort.
 
-  Goal elaborate_interpret map.empty <{ flatmap range(1, 10) "x" ["x"*"x"] }>
-     = Success (existT interp_type (TList TInt) [1; 4; 9; 16; 25; 36; 49; 64; 81]).
+  Goal run_program (init_locals ["a"]) <{
+     let "b" := 100 in
+     "a" <- 5 + "b";
+     "a" <- "a" + 1;
+  }> = Success [("a", existT interp_type TInt 106)].
+  reflexivity.  Abort.
+
+  Goal run_program (init_locals ["y"]) <{
+     let mut "a" := 2 in
+     "a" <- (let "x" := 5 in "x"*"a");
+     "y" <- "a"
+  }> = Success [("y", existT interp_type TInt 10)].
+  reflexivity. Abort.
+
+  Goal run_program (init_locals ["x"]) <{
+     "x" <- 5;
+     (let "y" := ("x" - 2) in
+         "x" <- "y" * 100
+     );
+  }> = Success [("x", existT interp_type TInt 300)].
+  reflexivity. Abort.
+
+  Goal run_program (init_locals ["o"]) <{
+     "o" <- let "x" := 2 in "x"
+  }> = Success [("o", existT _ TInt 2)].
   Proof. reflexivity. Abort.
+
+  Goal run_program (init_locals ["o"]) <{
+     "o" <- let "x" := 2 in "x"+3*100
+  }> = Success [("o", existT _ TInt 302)].
+  Proof. reflexivity. Abort.
+
+  Goal run_program (@set_local map.empty TBool "o" false) <{
+     "o" <- ! (1 == 1)
+  }> = Success [("o", existT _ TBool false)].
+  Proof. reflexivity. Abort.
+
+  Goal run_program (init_locals ["o"]) <{
+     "o" <- if !(1 == 2) then 5 else 98+1
+  }> = Success [("o", existT _ TInt 5)].
+  Proof. reflexivity. Abort.
+
+  Goal run_program (@set_local map.empty (TList TInt) "o" []) <{
+     "o" <- range(3, 5)
+  }> = Success [("o", existT _ (TList TInt) (3 :: 4 :: nil))].
+  Proof. reflexivity. Abort.
+
+  Goal run_program (@set_local map.empty (TList TInt) "o" []) <{
+     "o" <- flatmap [1, 2] "x" ["x"]
+  }> = Success [("o", existT _ (TList TInt) (1 :: 2 :: nil))].
+  reflexivity. Abort.
+
+  Goal run_program (@set_local map.empty (TList TInt) "o" []) <{
+     "o" <- flatmap [1] "x" ["x"]
+  }> = Success [("o", existT _ (TList TInt) (1 :: nil))].
+  reflexivity.  Abort.
+
+  Goal run_program (@set_local map.empty (TList TInt) "o" []) <{
+     "o" <- flatmap range(1, 10) "x" ["x"*"x"] }>
+     = Success [("o", existT interp_type (TList TInt) [1; 4; 9; 16; 25; 36; 49; 64; 81])].
+  Proof. reflexivity. Abort.
+
+  (* Program which test whether a number is square or not *)
+
+  Definition isSquare (n : Z) : pcommand := <{
+     let "n" := n in
+     for each "x" in range(0, "n"+1):
+         if "x"*"x" == "n"
+           then "ans" <- true
+           else skip
+           end;
+     end
+     }>.
+
+   Goal run_program (@set_local map.empty TBool "ans" false)
+      (isSquare 4) = Success [("ans", existT interp_type TBool true)].
+   Proof. reflexivity. Abort.
+
+   Goal run_program (@set_local map.empty TBool "ans" false)
+      (isSquare 25) = Success [("ans", existT interp_type TBool true)].
+   Proof. reflexivity. Abort.
+
+   Goal run_program (@set_local map.empty TBool "ans" false)
+      (isSquare (11*11 )) = Success [("ans", existT interp_type TBool true)].
+   Proof. reflexivity. Abort.
+
+   Goal run_program (@set_local map.empty TBool "ans" false)
+      (isSquare 0) = Success [("ans", existT interp_type TBool true)].
+   Proof. reflexivity. Abort.
+
+   Goal run_program (@set_local map.empty TBool "ans" false)
+      (isSquare 2) = Success [("ans", existT interp_type TBool false)].
+   Proof. reflexivity. Abort.
+
+   Goal run_program (@set_local map.empty TBool "ans" false)
+      (isSquare 13) = Success [("ans", existT interp_type TBool false)].
+   Proof. reflexivity. Abort.
+
+   Goal run_program (@set_local map.empty TBool "ans" false)
+      (isSquare (-2)) = Success [("ans", existT interp_type TBool false)].
+   Proof. reflexivity. Abort.
 
 End Examples.
 
