PyLevelLang/src/PyLevelLang/Interpret.v
@@ -125,6 +125,7 @@ Section WithMap.
                                          end
     | CGets x e => set_local l x (interp_expr l e)
     | CIf e c1 c2 => if interp_expr l e then interp_command l c1 else interp_command l c2
-    | CForeach x e c1 => fold_left (fun l' v => interp_command (set_local l' x v) c1) (interp_expr l e) l
+    | CForeach x e c1 =>
+        map.remove (fold_left (fun l' v => interp_command (set_local l' x v) c1) (interp_expr l e) l) x
     end.
 End WithMap.
